Ready to prove Lemma second_sentence! maybe need to check the lemma's statement again!

main.v
@@ -403,31 +403,206 @@ unfold Inc. unfold Included. intros f Hf. apply Hf.
 Qed.
 
     
-Lemma chain_finite_subset_has_maximum0 : forall (T D: Ensemble (Ensemble Formula)) (Gamma : Ensemble Formula),
+Lemma chain_finite_subset_has_maximum: forall (T D: Ensemble (Ensemble Formula)) (Gamma : Ensemble Formula),
 chain (Ensemble Formula) Inc (TheSet Gamma) T -> Included (Ensemble Formula) D T -> Finite (Ensemble Formula) D -> (exists (Gamma':(Ensemble Formula)), In (Ensemble Formula) D Gamma')
-->In (Ensemble Formula) D (UoCE1 D) /\ forall (Pi': Ensemble Formula), In (Ensemble Formula) D Pi' -> Inc Pi' (UoCE1 D).
+->exists (max : Ensemble Formula), In (Ensemble Formula) D max /\ (forall (Pi' : Ensemble Formula), In (Ensemble Formula) D Pi' -> Inc Pi' max).
 Proof.
-    Admitted.
+    intros T D Gamma H H0 H1 H2. apply finite_chain_has_maximum with (Gamma := Gamma).
+    +apply chain_subset_is_chain with (T:=T). 
+        ++apply H0.
+        ++apply H.
+    +apply H1.
+    +apply H2.
+Qed.
+    
 
 
 
 
 
 
+
+
+
+Lemma first_sentence : forall (T : Ensemble (Ensemble Formula)) (Pi : Ensemble Formula),
+Inc Pi (UoCE1 T) -> forall (f : Formula), In Formula Pi f -> exists (A : Ensemble Formula), In Formula A f /\ In (Ensemble Formula) T A.
+Proof.
+    intros T Pi HI f Hf. unfold UoCE1 in HI. unfold Inc in HI.
+    unfold Included in HI. apply HI in Hf. apply About_PropUoCEl in Hf.
+    unfold PropUoCE2 in Hf. destruct Hf as [A HA].
+    exists A. split. apply HA. apply HA.
+Qed.
+
+
+
+
+
+
+
+
+
+(*Includers of Pi elements:*)
+Definition PropIoPE (Pi : Ensemble Formula) (T : Ensemble (Ensemble Formula)) (A : Ensemble Formula) : Prop:=
+In (Ensemble Formula) T A /\ (exists (f : Formula), In Formula Pi f /\ In Formula A f /\ (forall (B : Ensemble Formula), In Formula B f -> In (Ensemble Formula) T B -> Inc A B)).
+
+Definition IoPE (Pi : Ensemble Formula) (T : Ensemble (Ensemble Formula)) : (Ensemble (Ensemble Formula)):=
+PropIoPE Pi T.
+
+Lemma About_IoPEr : forall (Pi A:Ensemble Formula) (T:Ensemble (Ensemble Formula)), 
+PropIoPE Pi T A -> In (Ensemble Formula) (IoPE Pi T) A.
+Proof. intros Pi A T H. apply H. 
+Qed.
+
+Lemma About_IoPEl : forall (Pi A:Ensemble Formula) (T:Ensemble (Ensemble Formula)), 
+In (Ensemble Formula) (IoPE Pi T) A -> PropIoPE Pi T A.
+Proof. intros f T H Q. apply Q.
+Qed.
+
+Lemma IoPE_Empty_set: forall (T : Ensemble (Ensemble Formula)), IoPE (Empty_set Formula) T = Empty_set (Ensemble Formula).
+Proof. intros T. apply Extensionality_Ensembles. unfold Same_set.
+split.
++unfold Included. intros X H. apply About_IoPEl in H. unfold PropIoPE in H.
+destruct H. destruct H0. rename x into f. destruct H0. destruct H0.
++unfold Included. intros f H. destruct H.
+Qed.
+
+Lemma IoPE_Singleton_set:forall (T : Ensemble (Ensemble Formula)) (f : Formula) (A: Ensemble Formula),
+In (Ensemble Formula)T A /\ In Formula A f /\ (forall (B:Ensemble Formula), In (Ensemble Formula) T B -> In Formula B f -> Inc A B)
+->IoPE (Singleton Formula f) T = Singleton (Ensemble Formula) A.
+intros T f A H. apply Extensionality_Ensembles. unfold Same_set.
+split. destruct H. destruct H0.
++unfold Included. intros X H2. apply About_IoPEl in H2. unfold PropIoPE in H2.
+assert (H3: X=A). destruct H2. destruct H3. destruct H3. destruct H4.
+-assert (H6 : Inc X A).
+--apply H5. ---apply Singleton_inv in H3. rewrite <- H3.
+apply H0.
+---apply H.
+--assert (Inc A X).
+---apply H1. ----apply H2. ----apply Singleton_inv in H3. rewrite -> H3.
+apply H4.
+---apply Extensionality_Ensembles. unfold Same_set. split.
+----apply H6. ----apply H7.
+-rewrite -> H3. apply In_singleton.
++destruct H. destruct H0. unfold Included. intros x H2.
+apply About_IoPEr. unfold PropIoPE. split.
+++apply Singleton_inv in H2. rewrite <- H2. apply H.
+++exists f. split.
++++apply In_singleton.
++++split.
+++++apply Singleton_inv in H2. rewrite <- H2. apply H0.
+++++intros B H3 H4. apply Singleton_inv in H2. rewrite <- H2.
+apply H1. -apply H4. -apply H3.
+Qed.
+
+
+Lemma Add_IoPE : forall (T : Ensemble (Ensemble Formula)) (Pi A': Ensemble Formula) (f:Formula), 
+~(In Formula Pi f) -> IoPE (Add Formula Pi f) T = Union (Ensemble Formula) (IoPE Pi T) (IoPE (Singleton Formula f) T).
+Proof.
+    intros T Pi A' f H.
+    apply Extensionality_Ensembles. unfold Same_set. split.
+    +unfold Included. unfold Add. intros A H1. apply About_IoPEl in H1.
+    unfold PropIoPE in H1. destruct H1. destruct H1. destruct H1.
+    apply Union_inv in H1. destruct H1.
+    ++apply Union_introl. apply About_IoPEr. unfold PropIoPE.
+    split.
+    -apply H0. -exists x. split. --apply H1. --apply H2.
+    ++apply Union_intror. apply Singleton_inv in H1. 
+    rewrite ->H1 in H. 
+    rewrite -> IoPE_Singleton_set with (A:=A).
+    +++apply In_singleton.
+    +++split.
+    -apply H0.
+    -split.
+    --rewrite -> H1. destruct H2. apply H2.
+    --intros B H3 H4. destruct H2. apply H5. 
+    ---rewrite <- H1. apply H4. ---apply H3.
+    +unfold Included. intros A H1. apply About_IoPEr. unfold PropIoPE.
+    apply Union_inv in H1. destruct H1.
+    ++split. apply About_IoPEl in H0. unfold PropIoPE in H0.
+    destruct H0. destruct H1. destruct H1. destruct H2.
+    +++apply H0.
+    +++destruct H0. destruct H1. destruct H1. destruct H2.
+    exists x. split. 
+    -apply Union_introl. apply H1.
+    -split. 
+    --apply H2.
+    --apply H3.
+    ++split.
+    -apply About_IoPEl in H0. unfold PropIoPE in H0.
+    destruct H0. destruct H1. destruct H1. destruct H2.
+    apply H0.
+    -apply About_IoPEl in H0. unfold PropIoPE in H0.
+    destruct H0. destruct H1. destruct H1. destruct H2.
+    exists x. split.
+    --apply Union_intror. apply H1.
+    --split. 
+    ---apply H2.
+    ---apply H3.
+    Qed.
 
     
-Lemma chain_finite_subset_has_maximum : forall (T D: Ensemble (Ensemble Formula)) (Gamma : Ensemble Formula),
-chain (Ensemble Formula) Inc (TheSet Gamma) T -> Included (Ensemble Formula) D T -> Finite (Ensemble Formula) D -> (exists (Gamma':(Ensemble Formula)), In (Ensemble Formula) D Gamma')
--> exists (Pi : Ensemble Formula), In (Ensemble Formula) D Pi /\ forall (Pi': Ensemble Formula), In (Ensemble Formula) D Pi' -> Inc Pi' Pi.
-Proof. intros T D Gamma H H0 H1 H2. destruct H2 as [Gamma' H2].
-Admitted.
+
+
+Lemma Union_finite_but_not_add : forall (U : Type) (A : Ensemble U) (x : U),
+Finite U A -> ~ In U A x -> Finite U (Union U A (Singleton U (x))).
+intros U A x H H3.
+assert (H1: Union U A (Singleton U x) = Add U A x).
++apply Extensionality_Ensembles. unfold Same_set.
+split.
+++unfold Included. intros u Hu. unfold Add. apply Hu.
+++unfold Included. intros u Hu. unfold Add in Hu. apply Hu.
++rewrite -> H1. apply Union_is_finite.
+-apply H.
+-apply H3.
+Qed.
+
+
+
+
+
+
+
+
+
+Lemma second_sentence : forall (T : Ensemble (Ensemble Formula)) (Pi : Ensemble Formula),
+(forall (f : Formula), In Formula Pi f -> exists (A : Ensemble Formula), In (Ensemble Formula) T A /\ In Formula A f) -> Finite Formula Pi -> Finite (Ensemble Formula) (IoPE Pi T).
+intros T Pi H H1.
+induction H1.
++rewrite IoPE_Empty_set. apply Empty_is_finite.
+
++rename A into Pi'. rewrite Add_IoPE.
+++apply Union_finite_but_not_add.
+++apply Pi'.
+++apply H0.
+
+
+
+
+
+assert (H1 :exists (n:nat), cardinal Formula Pi n /\ cardinal (Ensemble Formula) (IoPE Pi T) n).
++induction H.
+++exists 0. split. -apply card_empty. -unfold IoPE. 
+++
+
+
+
+
+
+
+
+
+
+
+
+
+
 
 
 
 Lemma UoCE1_has_subset : forall (T : Ensemble (Ensemble Formula)) (Gamma Pi: Ensemble Formula),
-chain (Ensemble Formula) Inc (TheSet Gamma) T /\ Inc Pi (UoCE1 T) /\ Finite Formula Pi 
+chain (Ensemble Formula) Inc (TheSet Gamma) T /\ Inc Pi (UoCE1 T) /\ Finite Formula Pi /\ (exists (f:Formula), In Formula Pi f)
 -> exists Pi', In (Ensemble Formula) T Pi' /\ Inc Pi Pi'.
-Proof. intros T Gamma Pi H. destruct H. destruct H0.    
+Proof. intros T Gamma Pi H.    
 Admitted.
 
 
@@ -473,7 +648,7 @@ Lemma Ex_of_Max1:forall (Gamma : Ensemble Formula),
     unfold Same_set. unfold Inc in H1. unfold Inc in H2. split. ---apply H1. --- apply H2.
     +intros T H1. exists (PropUoCE2 T) . unfold upper_bound. split.
     -intros X H2. unfold Inc. unfold Included. intros f.
-        intros H3. apply About_PropUoCE. unfold PropUoCE2.
+        intros H3. apply About_PropUoCEr. unfold PropUoCE2.
         exists X. split. --apply H2. --apply H3.
     -apply About_TheSet. split.
     --apply PropUoCE_Inclusion. ++ apply H1. 
